\documentclass[12pt,a4paper]{article}
\synctex=1
\usepackage[utf8]{inputenc}
\usepackage[margin=1cm]{geometry}
\usepackage{graphicx}
%\usepackage{verbatim}
\usepackage{amsmath}
\usepackage{amsfonts}
\usepackage{amssymb}
\usepackage{listings}
\usepackage{enumitem}
\usepackage{textcomp}
\usepackage{courier}
\usepackage{libertine}
\usepackage{pgfornament}
\usepackage{eso-pic}
\usepackage[hangul]{kotex}
\linespread{1.3}

\title{
	\centering
	\pgfornament[width=12cm,color=teal]{84}\\
	\vspace{1cm}
	\fontsize{50}{50} \selectfont {정보통신 수학 및 실습\\Homework}\\
		\pgfornament[width=12cm,color=teal]{88}\\
	\vfill}
\author{
	\LARGE
	\begin{tabular}{rl}
		\hline
		학번 : & 2016110056\\ 
		학과 : & 불교학부 \\
		이름 : & 박승원\\
		날짜 : & \today\\
		\hline
	\end{tabular}\vspace{2cm}
	\\
\includegraphics[width=0.5\textwidth]{logo.jpg}
	}
\date{}


\begin{document}
\maketitle
\pagenumbering{gobble}
\noindent
\lstset{language=matlab, columns=flexible, tabsize=4, frame=shadowbox, showstringspaces=false, breaklines=true, upquote=true, basicstyle=\normalsize}

\renewcommand{\thesubsubsection}{\alph{subsubsection})}
\renewcommand{\thesubsection}{\arabic{subsection}.}
\newpage

\section*{Chapter 9 Homework}
\subsection{Solve the Laplace transformations of the following functions using the tables. } 
\subsubsection{$L[5]$}
$
\displaystyle
\int_0^{\infty}5e^{-st}dt = \left[\frac{5}{-s}e^{-st}\right]_0^\infty
=\frac{5}{s}
$
\subsubsection{$L[5e^{-3t}]$}
$\displaystyle
\int_0^\infty 5e^{-3t}e^{-st}dt=\int_0^\infty 5e^{-(s+3)t}dt=\frac{5}{s+3}
$
\subsubsection{$L[cos(5t)]$}
$\displaystyle
cos5t = \frac{cos5t + isin5t + cos(-5t)+ isin(-5t)}{2}
=\frac{e^{i5t}+e^{-i5t}}{2}\\
\int_0^\infty cos(5t)e^{-st}dt=\frac{1}{2}\int_{0}^{\infty}(e^{i5t}+e^{-i5t})e^{-st}dt
=\frac{1}{2}\int_{0}^{\infty}(e^{(i5-s)t}+e^{(-i5-s)t})dt
=\frac{1}{2}\left[\frac{e^{(5i-s)t}}{5i-s}-\frac{e^{-(s+5i)t}}{s+5i}\right]_0^\infty=\frac{1}{2}(\frac{1}{-s+5i}-\frac{1}{s+5i})=\frac{s}{s^2+25}
$
\subsubsection{$L[5e^{-3t}cos(5t+1)]$}
$\displaystyle
\int_0^\infty 5e^{-3t}\frac{e^{i(5t+1)}+e^{-i(5t+1)}}{2}e^{-st}dt
=\frac{5}{2}\int_0^\infty e^{(5i-s-3)t+i}+e^{(-5i-s-3)t-i}dt
=\frac{5}{2}\left[\frac{e^{(5i-s-3)t+i}}{5i-s-3}+\frac{e^{(-5i-s-3)t-i}}{-5i-s-3}\right]_0^\infty
=\frac{5}{2}(-\frac{e^i}{5i-s-3}-\frac{e^{-i}}{-5i-s-3})
$
\subsubsection{$L[sin(5t)]$}
$\displaystyle
sin5t = -\frac{i}{2}(cos5t+isin5t-(cos(-5t)+isin(-5t)))
=-\frac{i}{2}(e^{i5t}-e^{-i5t})\\
\int_0^\infty sin(5t)e^{-3t}dt=\int_0^\infty -\frac{i}{2}(e^{i5t}-e^{-i5t})e^{-3t}dt
$
\subsubsection{$L[t^2sin(2t)]$}
$\displaystyle
\int_0^\infty t^2sin(2t)dt=-\frac{i}{2}\int_0^\infty t^2(e^{i2t}-e^{-i2t})dt
=\\
(e^{i2t}t^2)'=2ie^{i2t}t^2+e^{i2t}2t\\
e^{i2t}t^2=2\int e^{i2t}t^2 + e^{i2t}\\
\therefore \int e^{i2t}t^2 = \frac{e^{i2t}(t^2-1)}{2}\\
t \leftarrow -t : \int e^{-i2t}t^2 = \frac{e^{-i2t}(t^2-1)}{2}\\
-\frac{i}{2}\left[\frac{e^{i2t}(t^2-1)}{2} - \frac{e^{-i2t}(t^2-1)}{2}\right]_0^\infty=-\frac{i}{2}
$
\subsubsection{$L[\dfrac{d}{dt}sin(6t)]$}
$\displaystyle
(f(x)e^{-st})' = f'(x)e^{-st}+f(x)\cdot -se^{-st}\\
\int\frac{d}{dt}f(x)e^{-st}dt=f(x)e^{-st}+s\int f(x)e^{-st}\\
\therefore L[\dfrac{d}{dt}sin(6t)]=sin(6t)e^{-st}+s\int sin(6t)e^{-st}dt
$
\subsubsection{$L[\int_0^tydt]$}
$\displaystyle 
F(t)=\int_0^t f(u)du\\
\int_0^\infty \int_0^t f(u)du \cdot e^{-st}dt = 
\left[\int_0^t f(u)du\cdot \frac{e^{-st}}{-s}\right]_0^\infty 
- \int_0^\infty f(t)\frac{e^{-st}}{-s}dt = \frac{F(s)}{s}=\frac{1}{s^3}\\
\because L[y] = \dfrac{1}{s^2}
$
\subsubsection{$L[u(t-1)-u(t-2)]$}
$\displaystyle =\int_1^2 e^{-st}dt=\left[\frac{e^{-st}}{-s}\right]_1^2$
\subsubsection{$L[e^{-2t}u(t-2)]$}
$\displaystyle = \int_2^\infty e^{-(2+s)t}dt=\left[\frac{e^{-(2+s)t}}{-2-s}\right]_2^\infty$
\subsubsection{$L[6e^{-2.7t}cos(9.2t+3)]$}
$\displaystyle L[\cos (9.2t)] = \frac{9.2}{s^2+9.2^2}\\
L[6e^{-2.7t}cos(9.2t+3)]=\frac{9.2\times 6}{(s+2.7)^2+9.2^2}$
\subsection{Solve the inverse Laplace transformations using the tables..}
\subsubsection{$L^{-1}[\dfrac{5}{s+1}]$}
$5e^{-t}$
\subsubsection{$L^{-1}[\dfrac{6}{s^2}]$}
$6t$
\subsubsection{$L^{-1}[\dfrac{s+2}{(s+3)(s+4)}]$}
$\dfrac{-1}{s+3}+\dfrac{2}{s+4}\longrightarrow -e^{-3t}+2e^{-4t}$
\subsubsection{$L^{-1}[\dfrac{6}{-s^2+6}]$}
$-\dfrac{\sqrt{6}}{2}(\dfrac{1}{s+\sqrt{6}}-\dfrac{1}{s-\sqrt{6}})
\longrightarrow -\dfrac{\sqrt{6}}{2}(e^{-\sqrt{6}t} - e^{\sqrt{6}t})$
\subsubsection{$L^{-1}[\dfrac{5}{s}(1-e^{-4.5s})]$}
$\displaystyle L[f(x)g(x)] = F(s)G(s)\\
L^{-1}\left[\dfrac{5}{s} \right]= 5\\
\therefore \delta (t) - \frac{5}{s+4.5}$
\subsubsection{$L^{-1}[\dfrac{4+3j}{s+1-2j}+\dfrac{4-3j}{s+1+2j}]$}
$\displaystyle 2|A|e^{-\alpha t}cos(\beta t + \theta) = 
\frac{A}{s+\alpha - \beta j}+\frac{\bar{A}}{s+\alpha + \ beta j}\\
10e^{-t}\cos (2t)$
\subsubsection{$L^{-1}[\dfrac{6}{4s^2+20s+24}]$}
$\displaystyle \frac{6}{4(s+2)(s+3)}
=\frac{3}{2}(\frac{1}{s+2}-\frac{1}{s+3})\\
\therefore \frac{3}{2}(e^{-2t} - e^{-3t})$
\subsection{Solve the inverse Laplace transformations using partial fractions and the tables}
\subsubsection{$L^{-1}[\dfrac{1}{s^2-8s+25}]$}
$\displaystyle \frac{1}{(s-4-3j)(s-4+3j)}=
\frac{a+bj}{s-4-3j}+\frac{a-bj}{s-4+3j}\\
 a=0, b=-\frac{1}{6}\\
 \therefore \frac{1}{3}e^{-3t}cos(4t)$
\subsubsection{$L^{-1}[\dfrac{9s+4}{(s+3)^3}]$}
$\displaystyle \dfrac{9s+27-23}{(s+3)^3}=
\frac{9}{(s+3)^2}+\frac{-23}{(s+3)^3}\\
\therefore 9te^{-3t}-\frac{23}{2}t^2e^{-3t}$
\subsection{Find the system transfer functions of the following DE's.}
\subsubsection{$5\dfrac{d^2y}{dt^2}+6\dfrac{dy}{dt}+2y=5x(t)$}
$5s^2Y(s)+6sY(s) + 2Y(s) = 5X(s)\\
\therefore \dfrac{5}{5s^2+6s+2}$
\subsubsection{$\dfrac{dy}{dt}+8y=3x$}
$sY(s) + 8Y(s) = 3X(s)\\
\therefore \dfrac{3}{s+8}$
\end{document}
